Better formalization of Hochstein/Lamport example

HochsteinLamport.thy
@@ -4,80 +4,95 @@ begin
 
 (* see https://lorinhochstein.wordpress.com/2018/12/27/inductive-invariants/ *)
 
+datatype Pc = Start | SetX | Finish
+
 locale Algorithm =
   fixes N :: nat
   assumes Npos: "0 < N"
+  fixes pc :: "(nat \<Rightarrow> Pc) stfun"
   fixes x :: "(nat \<Rightarrow> nat) stfun"
-  fixes y :: "(nat \<Rightarrow> nat option) stfun"
-  assumes bvs: "basevars (x,y)"
+  fixes y :: "(nat \<Rightarrow> nat) stfun"
+  assumes bvs: "basevars (pc,x,y)"
   fixes Initial :: stpred
-  defines "Initial \<equiv> PRED (\<forall>n. id<x,#n> = #0 \<and> id<y,#n> = #None)"
+  defines "Initial \<equiv> PRED (\<forall>n. id<pc,#n> = #Start)"
   fixes Step1 :: "nat \<Rightarrow> action"
-  defines "Step1 n \<equiv> ACT (#n < #N \<and> id<$x,#n> = #0 \<and> id<x$,#n> = #1 \<and> (\<forall>n'. #n' \<noteq> #n \<longrightarrow> id<x$,#n'> = id<$x,#n'>) \<and> unchanged y)"
+  defines "Step1 n \<equiv> ACT (#n < #N
+    \<and> id<$pc,#n> = #Start \<and> id<pc$,#n> = #SetX
+    \<and> id<x$,#n> = #1
+    \<and> (\<forall>n'. #n' \<noteq> #n \<longrightarrow> id<pc$,#n'> = id<$pc,#n'>)
+    \<and> (\<forall>n'. #n' \<noteq> #n \<longrightarrow> id< x$,#n'> = id<$x ,#n'>)
+    \<and> unchanged y)"
   fixes Step2 :: "nat \<Rightarrow> nat \<Rightarrow> action"
-  defines "Step2 n j \<equiv> ACT (#n < #N \<and> #j < #N \<and> id<$x,#n> = #1 \<and> id<$y,#n> = #None \<and> id<y$,#n> = Some<id<$x,#j>> \<and> (\<forall>n'. #n' \<noteq> #n \<longrightarrow> id<y$,#n'> = id<$y,#n'>) \<and> unchanged x)"
+  defines "Step2 n j \<equiv> ACT (#n < #N \<and> #j < #N
+    \<and> id<$pc,#n> = #SetX \<and> id<pc$,#n> = #Finish
+    \<and> id<y$,#n> = id<$x,#j>
+    \<and> (\<forall>n'. #n' \<noteq> #n \<longrightarrow> id<pc$,#n'> = id<$pc,#n'>)
+    \<and> unchanged x
+    \<and> (\<forall>n'. #n' \<noteq> #n \<longrightarrow> id<y$,#n'> = id<$y,#n'>))"
   fixes Step :: action
   defines "Step \<equiv> ACT (\<exists> n. Step1 n \<or> (\<exists> j. Step2 n j))"
   fixes Spec :: temporal
-  defines "Spec \<equiv> TEMP (Init Initial \<and> \<box>[Step]_(x,y) \<and> WF(Step)_(x,y))"
+  defines "Spec \<equiv> TEMP (Init Initial \<and> \<box>[Step]_(pc,x,y) \<and> WF(Step)_(pc,x,y))"
 
 context Algorithm
 begin
 
-definition xSet :: "nat set stfun" where "xSet s \<equiv> { n. x s n = 1 }"
-definition ySet :: "nat set stfun" where "ySet s \<equiv> { n. y s n \<noteq> None }"
+definition xSet :: "nat set stfun" where "xSet s \<equiv> { n. pc s n \<noteq> Start }"
+definition ySet :: "nat set stfun" where "ySet s \<equiv> { n. pc s n = Finish }"
 
-lemma Step_cases[consumes 1, case_names stutter Step1 Step2]:
-  assumes sq_Step: "(s,t) \<Turnstile> [Step]_(x,y)"
-  assumes stutter: "\<lbrakk> x t = x s; y t = y s; xSet t = xSet s; ySet t = ySet s \<rbrakk> \<Longrightarrow> P"
-  assumes Step1: "\<And>n.   \<lbrakk> n < N;        x s n = 0;               x t n = 1;            \<forall> n'. n' \<noteq> n \<longrightarrow> x t n' = x s n'; y t = y s; xSet t = insert n (xSet s); ySet t = ySet s \<rbrakk> \<Longrightarrow> P"
-  assumes Step2: "\<And>n j. \<lbrakk> n < N; j < N; x s n = 1; y s n = None; y t n = Some (x s j); \<forall> n'. n' \<noteq> n \<longrightarrow> y t n' = y s n'; x t = x s; ySet t = insert n (ySet s); xSet t = xSet s \<rbrakk> \<Longrightarrow> P"
+lemma Step_cases[consumes 1, case_names unchanged Step1 Step2]:
+  assumes sq_Step: "(s,t) \<Turnstile> [Step]_(pc,x,y)"
+  assumes unchanged: "\<lbrakk> x t = x s; y t = y s; pc t = pc s; xSet t = xSet s; ySet t = ySet s \<rbrakk> \<Longrightarrow> P"
+  assumes Step1: "\<And>n.   \<lbrakk> n < N;        pc s n = Start; pc t n = SetX;   x t n = 1;     \<forall> n'. n' \<noteq> n \<longrightarrow> pc t n' = pc s n'; \<forall> n'. n' \<noteq> n \<longrightarrow> x t n' = x s n'; y t = y s; xSet t = insert n (xSet s); ySet t = ySet s \<rbrakk> \<Longrightarrow> P"
+  assumes Step2: "\<And>n j. \<lbrakk> n < N; j < N; pc s n = SetX;  pc t n = Finish; y t n = x s j; \<forall> n'. n' \<noteq> n \<longrightarrow> pc t n' = pc s n'; \<forall> n'. n' \<noteq> n \<longrightarrow> y t n' = y s n'; x t = x s; ySet t = insert n (ySet s); xSet t = xSet s \<rbrakk> \<Longrightarrow> P"
   shows P
 proof -
   from sq_Step consider
-    (stutter_case) "(s,t) \<Turnstile> unchanged (x,y)"
+    (unchanged_case) "(s,t) \<Turnstile> unchanged (pc,x,y)"
     | (Step1_case) "\<exists>n.   (s,t) \<Turnstile> Step1 n"
     | (Step2_case) "\<exists>n j. (s,t) \<Turnstile> Step2 n j"
     unfolding square_def Step_def by auto
   thus P
   proof cases
-    case stutter_case with stutter show P unfolding xSet_def ySet_def by simp
+    case unchanged_case with unchanged show P unfolding xSet_def ySet_def by simp
   next
     case Step1_case
     then obtain n where st: "(s,t) \<Turnstile> Step1 n" ..
-    thus P by (intro Step1 [of n], auto simp add: Step1_def xSet_def ySet_def)
+    thus P
+      apply (intro Step1 [of n], auto simp add: Step1_def xSet_def ySet_def)
+      using Pc.distinct by metis+
   next
     case Step2_case
     then obtain n j where st: "(s,t) \<Turnstile> Step2 n j" by blast
-    thus P by (intro Step2 [of n j], auto simp add: Step2_def xSet_def ySet_def)
+    thus P apply (intro Step2 [of n j], auto simp add: Step2_def xSet_def ySet_def)
+      using Pc.distinct by metis+
   qed
 qed
 
 definition Safety :: stpred
-  where "Safety s \<equiv> (\<forall> n. x s n \<in> {0, 1})
-                  \<and> (\<forall> n. y s n \<in> {None, Some 0, Some 1})
-                  \<and> xSet s \<subseteq> {n. n < N}
+  where "Safety s \<equiv> xSet s \<subseteq> {n. n < N}
                   \<and> ySet s \<subseteq> xSet s
-                  \<and> (ySet s = {n. n < N} \<longrightarrow> (\<exists> n < N. y s n = Some 1))"
+                  \<and> (\<forall> n \<in> xSet s. x s n = 1)
+                  \<and> (ySet s = {n. n < N} \<longrightarrow> (\<exists> n < N. y s n = 1))"
 
 lemma Safety: "\<turnstile> Spec \<longrightarrow> \<box>Safety"
 proof (intro invariantI)
   show "\<turnstile> Spec \<longrightarrow> Init Safety" using Npos by (auto simp add: Spec_def Safety_def Init_def Initial_def xSet_def ySet_def)
-  show "\<turnstile> Spec \<longrightarrow> \<box>[Step]_(x,y)" by (auto simp add: Spec_def)
+  show "\<turnstile> Spec \<longrightarrow> \<box>[Step]_(pc,x,y)" by (auto simp add: Spec_def)
 
   fix s t
   assume s_Safety: "s \<Turnstile> Safety"
-  assume "(s,t) \<Turnstile> [Step]_(x,y)"
+  assume "(s,t) \<Turnstile> [Step]_(pc,x,y)"
   thus "t \<Turnstile> Safety"
   proof (cases rule: Step_cases)
-    case stutter with s_Safety show ?thesis unfolding Safety_def by simp
+    case unchanged with s_Safety show ?thesis unfolding Safety_def by simp
   next
     case (Step1 n)
     show ?thesis
       unfolding Safety_def
-    proof (intro conjI allI impI exI)
-      from s_Safety Step1 show "x t n' \<in> {0, 1}" "y t n' \<in> {None, Some 0, Some 1}" for n' unfolding Safety_def apply simp_all by metis
-      from s_Safety Step1 show "xSet t \<subseteq> {n. n < N}" "ySet t \<subseteq> xSet t" unfolding Safety_def by auto
+    proof (intro conjI impI exI)
+      show "\<forall>n\<in>xSet t. x t n = 1" "xSet t \<subseteq> {n. n < N}" "ySet t \<subseteq> xSet t" "n < N"
+        using s_Safety Step1 unfolding Safety_def by fastforce+
 
       from Step1 have "ySet s = ySet t" by simp
       also assume "ySet t = {n. n < N}"
@@ -86,85 +101,90 @@ proof (intro invariantI)
       ultimately have "xSet s = {n. n < N}" by auto
       with Step1 have "n \<in> xSet s" by (auto simp add: xSet_def)
       with Step1 have False by (simp add: xSet_def)
-      thus "n < N" "y t n = Some 1" by simp_all
+      thus "y t n = 1" by simp_all
     qed
   next
     case (Step2 n j)
     show ?thesis
       unfolding Safety_def
-    proof (intro conjI allI impI exI)
-      from s_Safety Step2 show "x t n' \<in> {0, 1}" "y t n' \<in> {None, Some 0, Some 1}" for n' unfolding Safety_def apply simp_all by metis
-      from s_Safety Step2 show "xSet t \<subseteq> {n. n < N}" "ySet t \<subseteq> xSet t" unfolding Safety_def xSet_def ySet_def by auto
-      from Step2 show "n < N" by simp
+    proof (intro conjI impI exI)
+      show "\<forall>n\<in>xSet t. x t n = 1" "xSet t \<subseteq> {n. n < N}" "ySet t \<subseteq> xSet t" "n < N"
+        using s_Safety Step2 unfolding Safety_def xSet_def ySet_def by fastforce+
 
       assume "ySet t = {n. n < N}"
       with `ySet t \<subseteq> xSet t` `xSet t \<subseteq> {n. n < N}` have "xSet s = {n. n < N}" using Step2 by simp
-      with Step2 have "x s j = 1" unfolding xSet_def by auto
-      with Step2 show "y t n = Some 1" by simp
+      with Step2 s_Safety have "x s j = 1" unfolding Safety_def by auto
+      with Step2 show "y t n = 1" by simp
     qed
   qed
 qed
 
-lemma angle_Step_eq: "(ACT <Step>_(x, y)) = Step"
+lemma angle_Step_eq: "(ACT <Step>_(pc, x, y)) = Step"
 proof (intro ext iffI)
   fix st
-  show "st \<Turnstile> <Step>_(x,y) \<Longrightarrow> st \<Turnstile> Step" unfolding angle_def by auto
+  show "st \<Turnstile> <Step>_(pc,x,y) \<Longrightarrow> st \<Turnstile> Step" unfolding angle_def by auto
 
   assume Step: "st \<Turnstile> Step"
   obtain s t where st: "st = (s,t)" by fastforce
 
-  have "(s,t) \<Turnstile> <Step>_(x,y)"
+  have "(s,t) \<Turnstile> <Step>_(pc,x,y)"
     unfolding angle_def
   proof (intro temp_conjI)
     from Step st show "(s,t) \<Turnstile> Step" by simp
-    thus "(s,t) \<Turnstile> \<not> unchanged (x, y)"
+    thus "(s,t) \<Turnstile> \<not> unchanged (pc, x, y)"
       by (auto simp add: Step_def Step1_def Step2_def)
   qed
-  thus "st \<Turnstile> <Step>_(x,y)" by (simp add: st)
+  thus "st \<Turnstile> <Step>_(pc,x,y)" by (simp add: st)
 qed
 
 lemma enabled_StepI:
   assumes "s \<Turnstile> Safety"
   assumes "ySet s \<noteq> {n. n < N}"
   shows "s \<Turnstile> Enabled Step"
-proof (cases "xSet s = {n. n < N}")
-  case False
-  with assms obtain n where n: "n < N" "x s n = 0" unfolding xSet_def Safety_def by blast
-
-  show ?thesis unfolding Step_def enabled_ex [temp_use] enabled_disj [temp_use]
-  proof (intro exI [where x = n] disjI1, enabled bvs, intro exI allI impI, elim conjE)
-    fix u
-    assume "x u = (\<lambda>m. if m = n then 1 else x s m)" "y u = y s"
-    with n show "(s,u) \<Turnstile> Step1 n" by (auto simp add: Step1_def)
-  qed
-next
-  case True
-  from assms obtain n where n: "n < N" "y s n = None" unfolding ySet_def Safety_def by auto
-
-  show ?thesis unfolding Step_def enabled_ex [temp_use] enabled_disj [temp_use]
-  proof (intro exI [where x = n] disjI2, enabled bvs, intro exI allI impI, elim conjE)
-    fix u
-    assume xu: "x u = x s" and yu: "y u = (\<lambda>m. if m = n then Some (x s n) else y s m)"
-    with n True show "(s,u) \<Turnstile> Step2 n n" by (auto simp add: Step2_def xSet_def)
-  qed
+proof -
+  from assms obtain n where n: "n < N" "pc s n \<noteq> Finish" unfolding ySet_def Safety_def by auto
+  thus ?thesis
+  proof (cases "pc s n")
+    case Start
+    show ?thesis unfolding Step_def enabled_ex [temp_use] enabled_disj [temp_use]
+    proof (intro exI [where x = n] disjI1, enabled bvs, intro exI allI impI, elim conjE)
+      fix u
+      assume
+        "pc u = (\<lambda>m. if m = n then SetX else pc s m)"
+        "x  u = (\<lambda>m. if m = n then 1    else x s m)"
+        "y  u = y s"
+      with n Start show "(s,u) \<Turnstile> Step1 n" by (auto simp add: Step1_def)
+    qed
+  next
+    case SetX
+    show ?thesis unfolding Step_def enabled_ex [temp_use] enabled_disj [temp_use]
+    proof (intro exI [where x = n] disjI2, enabled bvs, intro exI allI impI, elim conjE)
+      fix u
+      assume
+        "pc u = (\<lambda>m. if m = n then Finish else pc s m)"
+        "y  u = (\<lambda>m. if m = n then x s n else y s m)"
+        "x  u = x s"
+      with n SetX show "(s,u) \<Turnstile> Step2 n n" by (auto simp add: Step2_def)
+    qed
+  qed simp
 qed
 
 lemma StepFair:
-  assumes "\<turnstile> $P \<and> $Safety \<and> [Step]_(x,y) \<longrightarrow> P$ \<or> Q$"
+  assumes "\<turnstile> $P \<and> $Safety \<and> [Step]_(pc,x,y) \<longrightarrow> P$ \<or> Q$"
   assumes "\<turnstile> $P \<and> $Safety \<and>  Step        \<longrightarrow>      Q$"
-  assumes "\<turnstile> $P \<and> $Safety \<and> [Step]_(x,y) \<longrightarrow> $Enabled Step"
+  assumes "\<turnstile> $P \<and> $Safety \<and> [Step]_(pc,x,y) \<longrightarrow> $Enabled Step"
   shows "\<turnstile> Spec \<longrightarrow> (P \<leadsto> Q)"
 proof -
-  from Safety have "\<turnstile> Spec \<longrightarrow> \<box>([Step]_(x,y) \<and> $Safety) \<and> WF(Step)_(x,y)" by (auto simp add: Spec_def more_temp_simps)
-  also have "\<turnstile> \<box>([Step]_(x,y) \<and> $Safety) \<and> WF(Step)_(x,y) \<longrightarrow> (P \<leadsto> Q)"
+  from Safety have "\<turnstile> Spec \<longrightarrow> \<box>([Step]_(pc,x,y) \<and> $Safety) \<and> WF(Step)_(pc,x,y)" by (auto simp add: Spec_def more_temp_simps)
+  also have "\<turnstile> \<box>([Step]_(pc,x,y) \<and> $Safety) \<and> WF(Step)_(pc,x,y) \<longrightarrow> (P \<leadsto> Q)"
     using assms angle_Step_eq by (intro WF1, auto)
   finally show ?thesis .
 qed
 
 lemma StepFair_action:
-  assumes "\<And>s t. \<lbrakk> s \<Turnstile> P; s \<Turnstile> Safety; (s,t) \<Turnstile> [Step]_(x,y) \<rbrakk> \<Longrightarrow> t \<Turnstile> P \<or> Q"
-  assumes "\<And>s t. \<lbrakk> s \<Turnstile> P; s \<Turnstile> Safety; (s,t) \<Turnstile>  Step        \<rbrakk> \<Longrightarrow> t \<Turnstile>     Q"
-  assumes "\<And>s t. \<lbrakk> s \<Turnstile> P; s \<Turnstile> Safety; (s,t) \<Turnstile> [Step]_(x,y) \<rbrakk> \<Longrightarrow> s \<Turnstile> Enabled Step"
+  assumes "\<And>s t. \<lbrakk> s \<Turnstile> P; s \<Turnstile> Safety; (s,t) \<Turnstile> [Step]_(pc,x,y) \<rbrakk> \<Longrightarrow> t \<Turnstile> P \<or> Q"
+  assumes "\<And>s t. \<lbrakk> s \<Turnstile> P; s \<Turnstile> Safety; (s,t) \<Turnstile>  Step           \<rbrakk> \<Longrightarrow> t \<Turnstile>     Q"
+  assumes "\<And>s t. \<lbrakk> s \<Turnstile> P; s \<Turnstile> Safety; (s,t) \<Turnstile> [Step]_(pc,x,y) \<rbrakk> \<Longrightarrow> s \<Turnstile> Enabled Step"
   shows "\<turnstile> Spec \<longrightarrow> (P \<leadsto> Q)"
   using assms by (intro StepFair actionI, auto)
 
@@ -194,16 +214,15 @@ proof -
           and s_F: "s \<Turnstile> F xsys" unfolding F_def by auto
 
         assume Safety: "s \<Turnstile> Safety"
-        hence x_range: "\<And>n. x s n \<in> {0, 1}" and y_range: "\<And>n. y s n \<in> {None, Some 0, Some 1}" 
-          and xSet_range: "xSet s \<subseteq> {n. n < N}" and ySet_range: "ySet s \<subseteq> {n. n < N}"
-          and ySet_xSet: "ySet s \<subseteq> xSet s" 
+        hence xSet_range: "xSet s \<subseteq> {n. n < N}" and ySet_range: "ySet s \<subseteq> {n. n < N}"
+          and ySet_xSet: "ySet s \<subseteq> xSet s" and xSet_set: "\<And>n. n \<in> xSet s \<Longrightarrow> x s n = 1"
           unfolding Safety_def by auto
 
         show "s \<Turnstile> Enabled Step" by (intro enabled_StepI Safety running)
 
         show progress: "t \<Turnstile> ySet = #{n. n < N} \<or> (\<exists>y. #((y, xsys) \<in> r) \<and> F y \<and> ySet \<noteq> #{n. n < N})" if Step: "(s,t) \<Turnstile> Step"
         proof -
-          from Step have "(s,t) \<Turnstile> [Step]_(x,y)" unfolding square_def by simp
+          from Step have "(s,t) \<Turnstile> [Step]_(pc,x,y)" unfolding square_def by simp
           thus ?thesis
           proof (cases rule: Step_cases)
             case (Step1 n)
@@ -223,19 +242,27 @@ proof -
                 from False show "t \<Turnstile> ySet \<noteq> #{n. n < N}" by simp
                 from Step2 xs ys show "t \<Turnstile> F (xs, ys - {n})" unfolding F_def by auto
                 from Step2 xs ys show "t \<Turnstile> (#(((xs, ys - {n}), xsys) \<in> r))"
-                  unfolding r_def xsys apply simp
-                  by (metis (mono_tags, lifting) Diff_iff mem_Collect_eq psubsetI singletonI subsetI ySet_def)
+                  unfolding r_def xsys
+                proof simp
+                  assume a1: "pc s n = SetX"
+                  assume "n < N"
+                  then have "n \<in> {n. n < N} - ySet s"
+                    using a1 by (simp add: ySet_def)
+                  then show "{n. n < N} - ySet s - {n} \<subset> {n. n < N} - ySet s"
+                    by blast
+                qed
+
               qed
               then show ?thesis by auto
             qed
           next
-            case stutter
-            from Step have "(s,t) \<Turnstile> <Step>_(x,y)" unfolding angle_Step_eq.
-            with stutter show ?thesis by (simp add: angle_def)
+            case unchanged
+            from Step have "(s,t) \<Turnstile> <Step>_(pc,x,y)" unfolding angle_Step_eq.
+            with unchanged show ?thesis by (simp add: angle_def)
           qed
         qed
 
-        assume "(s,t) \<Turnstile> [Step]_(x,y)"
+        assume "(s,t) \<Turnstile> [Step]_(pc,x,y)"
         then consider (Step) "(s,t) \<Turnstile> Step" | (unchanged) "x t = x s" "y t = y s" "xSet t = xSet s" "ySet t = ySet s" unfolding square_def xSet_def ySet_def by auto
         thus "t \<Turnstile> F xsys \<and> ySet \<noteq> #{n. n < N} \<or> ySet = #{n. n < N} \<or> (\<exists>y. #((y, xsys) \<in> r) \<and> F y \<and> ySet \<noteq> #{n. n < N})"
         proof cases
@@ -253,21 +280,21 @@ qed
 
 lemma Termination_stops: "\<turnstile> Spec \<longrightarrow> \<diamond>\<box>(ySet = #{n. n < N})"
 proof (intro stable_dmd_stuck Termination)
-  from Safety have "\<turnstile> Spec \<longrightarrow> \<box>([Step]_(x,y) \<and> $Safety)" unfolding Spec_def
+  from Safety have "\<turnstile> Spec \<longrightarrow> \<box>([Step]_(pc,x,y) \<and> $Safety)" unfolding Spec_def
     apply auto using Init_stp_act_rev boxInit_act boxInit_stp by auto
-  also have "\<turnstile> \<box>([Step]_(x,y) \<and> $Safety) \<longrightarrow> stable (ySet = #{n. n < N})"
+  also have "\<turnstile> \<box>([Step]_(pc,x,y) \<and> $Safety) \<longrightarrow> stable (ySet = #{n. n < N})"
   proof (intro StableT actionI temp_impI, elim temp_conjE, simp_all)
     fix s t
-    assume "(s,t) \<Turnstile> [Step]_(x, y)" "ySet s = {n. n < N}" "Safety s"
+    assume "(s,t) \<Turnstile> [Step]_(pc,x,y)" "ySet s = {n. n < N}" "Safety s"
     thus "ySet t = {n. n < N}" by (cases rule: Step_cases, auto)
   qed
   finally show "\<turnstile> Spec \<longrightarrow> stable (ySet = #{n. n < N})".
 qed
 
-lemma eventually_1: "\<turnstile> Spec \<longrightarrow> \<diamond>(\<exists>n. id<y,#n> = #(Some 1))"
+lemma eventually_1: "\<turnstile> Spec \<longrightarrow> \<diamond>(\<exists>n. id<y,#n> = #1)"
 proof -
   note Termination
-  also have "\<turnstile> Spec \<longrightarrow> ((ySet = #{n. n < N}) \<leadsto> (\<exists>n. id<y,#n> = #(Some 1)))"
+  also have "\<turnstile> Spec \<longrightarrow> ((ySet = #{n. n < N}) \<leadsto> (\<exists>n. id<y,#n> = #1))"
     by (intro imp_INV_leadsto [OF Safety imp_imp_leadsto] intI temp_impI, elim temp_conjE, auto simp add: Safety_def)
   finally show ?thesis .
 qed
